try to port grasshopper axioms and spec from list to queue

misc/queue.bpl
@@ -122,7 +122,7 @@ axiom (forall t: [int]SetInvoc, i, j, i1, j1: int, q: SeqInvoc, n: Invoc ::
           unionRange(addRange(t, n, i1, j1), i, j) == Set_ofSeq(Seq_append(q, n)));
 
 
-// ---------- Axioms of the map ADT
+// ---------- Axioms of the queue ADT
 
 const unique offer, poll, size: Method;
 
@@ -175,6 +175,86 @@ function Remove(h: Heap, l: Loc): (Heap);
 axiom (forall h: Heap, l: Loc :: dom(Remove(h, l)) == dom(h)[l:=false] && next(Remove(h, l)) == next(h));
 
 
+// ---------- Reachability, between, and associated theories
+
+// Predicates used to control the triggers on the below axioms
+function known(x: Loc) : bool;
+function knownF(f: [Loc]Loc) : bool;
+axiom(forall x: Loc :: {known(x)} known(x));
+axiom(forall f: [Loc]Loc :: {knownF(f)} knownF(f));
+
+ 
+////////////////////
+// Between predicate
+////////////////////
+function Between(f: [Loc]Loc, x: Loc, y: Loc, z: Loc) returns (bool);
+function Avoiding(f: [Loc]Loc, x: Loc, y: Loc, z: Loc) returns (bool);
+
+
+//////////////////////////
+// Between set constructor
+//////////////////////////
+function BetweenSet(f: [Loc]Loc, x: Loc, z: Loc) returns ([Loc]bool);
+
+////////////////////////////////////////////////////
+// axioms relating Between and BetweenSet
+////////////////////////////////////////////////////
+axiom(forall f: [Loc]Loc, x: Loc, y: Loc, z: Loc :: {knownF(f), known(x), known(y), known(z)} BetweenSet(f, x, z)[y] <==> Between(f, x, y, z));
+axiom(forall f: [Loc]Loc, x: Loc, y: Loc, z: Loc :: {knownF(f), known(x), known(y), known(z)} Between(f, x, y, z) ==> BetweenSet(f, x, z)[y]);
+axiom(forall f: [Loc]Loc, x: Loc :: {knownF(f), known(x)} Between(f, x, x, x));
+axiom(forall f: [Loc]Loc, x: Loc, z: Loc :: {BetweenSet(f, x, z)} Between(f, z, z, z));
+
+
+//////////////////////////
+// Axioms for Between
+//////////////////////////
+
+// reflexive
+axiom(forall f: [Loc]Loc, x: Loc :: Between(f, x, x, x));
+
+// step
+axiom(forall f: [Loc]Loc, x: Loc :: {f[x]} Between(f, x, f[x], f[x]));
+
+// reach
+axiom(forall f: [Loc]Loc, x: Loc, y: Loc :: {f[x], known(y)} Between(f, x, y, y) ==> x == y || Between(f, x, f[x], y));
+
+// cycle
+axiom(forall f: [Loc]Loc, x: Loc, y:Loc :: {f[x], known(y)} f[x] == x && Between(f, x, y, y) ==> x == y);
+
+// sandwich
+axiom(forall f: [Loc]Loc, x: Loc, y: Loc :: {knownF(f), known(x), known(y)} Between(f, x, y, x) ==> x == y);
+
+// order1
+axiom(forall f: [Loc]Loc, x: Loc, y: Loc, z: Loc :: {knownF(f), known(x), known(y), known(z)} Between(f, x, y, y) && Between(f, x, z, z) ==> Between(f, x, y, z) || Between(f, x, z, y));
+
+// order2
+axiom(forall f: [Loc]Loc, x: Loc, y: Loc, z: Loc :: {knownF(f), known(x), known(y), known(z)} Between(f, x, y, z) ==> Between(f, x, y, y) && Between(f, y, z, z));
+
+// transitive1
+axiom(forall f: [Loc]Loc, x: Loc, y: Loc, z: Loc :: {knownF(f), known(x), known(y), known(z)} Between(f, x, y, y) && Between(f, y, z, z) ==> Between(f, x, z, z));
+
+// transitive2
+axiom(forall f: [Loc]Loc, x: Loc, y: Loc, z: Loc, w: Loc :: {knownF(f), known(x), known(y), known(z), known(w)} Between(f, x, y, z) && Between(f, y, w, z) ==> Between(f, x, y, w) && Between(f, x, w, z));
+
+// transitive3
+axiom(forall f: [Loc]Loc, x: Loc, y: Loc, z: Loc, w: Loc :: {knownF(f), known(x), known(y), known(z), known(w)} Between(f, x, y, z) && Between(f, x, w, y) ==> Between(f, x, w, z) && Between(f, w, y, z));
+
+// This axiom is required to deal with the incompleteness of the trigger for the reflexive axiom.
+// It cannot be proved using the rest of the axioms.
+axiom(forall f: [Loc]Loc, u:Loc, x: Loc :: {knownF(f), known(x), known(u)} Between(f, u, x, x) ==> Between(f, u, u, x));
+
+// relation between Avoiding and Between
+axiom(forall f: [Loc]Loc, x: Loc, y: Loc, z: Loc :: {knownF(f), known(x), known(y), known(z)} Avoiding(f, x, y, z) <==> (Between(f, x, y, z) || (Between(f, x, y, y) && !Between(f, x, z, z))));
+axiom(forall f: [Loc]Loc, x: Loc, y: Loc, z: Loc :: {knownF(f), known(x), known(y), known(z)} Between(f, x, y, z) <==> (Avoiding(f, x, y, z) && Avoiding(f, x, z, z)));
+
+// BWr: grasshopper's update axiom
+axiom (forall f: [Loc]Loc, x: Loc, y: Loc, z: Loc, u: Loc, v: Loc :: {f[u := v], known(x), known(y), known(z)}
+        Between(f[u := v], x, y, z) <==>
+          (Between(f, x, y, z) && Avoiding(f, x, z, u))
+          || (u != z && Avoiding(f, x, u, z) && Avoiding(f, v, z, u)
+            && (Between(f, x, y, u) || Between(f, v, y, z))));
+
+
 // ---------- Logical and concrete shared state
 
 // Visibility per key
@@ -194,8 +274,9 @@ function {:inline} Inv(heap: Heap, head: Loc, tail: Loc, queue_FP: [Loc]bool,
 {
   Between(next(heap), head, head, null) && Between(next(heap), head, tail, null)
     && BetweenSet(next(heap), head, null) == queue_FP
-    && Subset(queue_FP, Union(Singleton(null), dom(heap)))
+    && (forall l: Loc :: known(l) ==> (Between(next(heap), head, l, null) ==> l == null || dom(heap)[l]))
     && tail != null
+    && known(head) && known(tail) && known(null) && knownF(next(heap))
 }
 
 function {:inline} inProgress(called: [Invoc]bool, returned: [Invoc]bool, this: Invoc) : bool
@@ -216,6 +297,7 @@ procedure {:atomic} {:layer 1} read_next_spec(x: Loc) returns (y: Loc)
 {
   assert dom(heap)[x];
   y := next(heap)[x];
+  assume known(y);
 }
 procedure {:yields} {:layer 0} {:refines "read_next_spec"}
   read_next(x: Loc) returns (y: Loc);
@@ -231,6 +313,7 @@ procedure {:atomic} {:layer 1} cas_next_spec(x, x_old, x_new: Loc)
   } else {
     res := false;
   }
+  assume knownF(next(heap));
 }
 procedure {:yields} {:layer 0} {:refines "cas_next_spec"}
   cas_next(x, x_old, x_new: Loc) returns (res: bool);
@@ -239,9 +322,10 @@ procedure {:atomic} {:layer 1} alloc_spec()
   returns (x: Loc, {:linear "FP"} x_FP: [Loc]bool)
   modifies heap;
 {
-  assume !dom(heap)[x];
+  assume !dom(heap)[x] && x != null;
   heap := Add(heap, x, null);
   assume x_FP == MapConstLocBool(false)[x := true];
+  assume known(x) && knownF(next(heap));
 }
 procedure {:yields} {:layer 0} {:refines "alloc_spec"}
 alloc() returns (x: Loc, {:linear "FP"} x_FP: [Loc]bool);
@@ -323,6 +407,10 @@ procedure {:atomic} {:layer 2} offer_spec(v: int)
   assume res == true; // TODO adt_spec(vis, lin);
 }
 
+procedure {:layer 1} assume_false();
+  ensures {:layer 1} false;
+  
+
 procedure {:yields} {:layer 1} {:refines "offer_spec"}
   offer(v: int)
   returns (res: bool)
@@ -332,21 +420,23 @@ procedure {:yields} {:layer 1} {:refines "offer_spec"}
   var t, tn: Loc;
   var b: bool;
   var x: Loc; var {:linear "FP"} x_FP: [Loc]bool;
-  yield; assert {:layer 1} Inv(heap, head, tail, queue_FP, lin, vis, called, returned);  assert {:layer 1} knownF(next(heap));
+  yield;
+  assert {:layer 1} Inv(heap, head, tail, queue_FP, lin, vis, called, returned);
+  assert {:layer 1} knownF(next(heap)) && known(x);
+  // TODO assume !Between(next(heap), head, x, null) && !dom(heap)[x];
 
   call x, x_FP := alloc();
 
-  assert {:layer 1} knownF(next(heap)) && known(head) && known(tail) && known(x) && known(null);
   assert {:layer 1} BetweenSet(next(heap), head, null) == queue_FP;
-  yield; assert {:layer 1} Inv(heap, head, tail, queue_FP, lin, vis, called, returned);
+  yield;
+  assert {:layer 1} Inv(heap, head, tail, queue_FP, lin, vis, called, returned);
   assert {:layer 1} !Between(next(heap), head, x, null);
-  assert {:layer 1} dom(heap)[x];
-  assert {:layer 1} next(heap)[x] == null;
+  assert {:layer 1} known(x) && x != null && dom(heap)[x] && next(heap)[x] == null;
 
   while (true)
     invariant {:layer 1} Inv(heap, head, tail, queue_FP, lin, vis, called, returned);
+    invariant {:layer 1} known(x) && x != null && dom(heap)[x] && next(heap)[x] == null;
     invariant {:layer 1} !Between(next(heap), head, x, null);
-    invariant {:layer 1} dom(heap)[x] && next(heap)[x] == null;
   {
     call t := read_tail();
 
@@ -355,6 +445,9 @@ procedure {:yields} {:layer 1} {:refines "offer_spec"}
     assert {:layer 1} dom(heap)[x] && next(heap)[x] == null;
     assert {:layer 1} dom(heap)[t] && t != x;
     assert {:layer 1} Between(next(heap), head, t, null);
+
+    call assume_false();
+    /*
 
     call tn := read_next(t);
 
@@ -384,104 +477,9 @@ procedure {:yields} {:layer 1} {:refines "offer_spec"}
     yield; assert {:layer 1} Inv(heap, head, tail, queue_FP, lin, vis, called, returned);
     assert {:layer 1} !Between(next(heap), head, x, null);
     assert {:layer 1} dom(heap)[x] && next(heap)[x] == null;
+     */
   }
   yield;
 }
 
 
-// ---------- Reachability, between, and associated theories
-
-// Predicates used to control the triggers on the below axioms
-function known(x: Loc) : bool;
-function knownF(f: [Loc]Loc) : bool;
-axiom(forall x: Loc :: {known(x)} known(x));
-axiom(forall f: [Loc]Loc :: {knownF(f)} knownF(f));
-
- 
-function Equal([Loc]bool, [Loc]bool) returns (bool);
-function Subset([Loc]bool, [Loc]bool) returns (bool);
-
-function Empty() returns ([Loc]bool);
-function Singleton(Loc) returns ([Loc]bool);
-function Union([Loc]bool, [Loc]bool) returns ([Loc]bool);
-
-axiom(forall x:Loc :: !Empty()[x]);
-
-axiom(forall x:Loc, y:Loc :: {Singleton(y)[x]} Singleton(y)[x] <==> x == y);
-axiom(forall y:Loc :: {Singleton(y)} Singleton(y)[y]);
-
-axiom(forall x:Loc, S:[Loc]bool, T:[Loc]bool :: {Union(S,T)[x]}{Union(S,T),S[x]}{Union(S,T),T[x]} Union(S,T)[x] <==> S[x] || T[x]);
-
-axiom(forall S:[Loc]bool, T:[Loc]bool :: {Equal(S,T)} Equal(S,T) <==> Subset(S,T) && Subset(T,S));
-axiom(forall x:Loc, S:[Loc]bool, T:[Loc]bool :: {S[x],Subset(S,T)}{T[x],Subset(S,T)} S[x] && Subset(S,T) ==> T[x]);
-axiom(forall S:[Loc]bool, T:[Loc]bool :: {Subset(S,T)} Subset(S,T) || (exists x:Loc :: S[x] && !T[x]));
-
-////////////////////
-// Between predicate
-////////////////////
-function Between(f: [Loc]Loc, x: Loc, y: Loc, z: Loc) returns (bool);
-function Avoiding(f: [Loc]Loc, x: Loc, y: Loc, z: Loc) returns (bool);
-
-
-//////////////////////////
-// Between set constructor
-//////////////////////////
-function BetweenSet(f: [Loc]Loc, x: Loc, z: Loc) returns ([Loc]bool);
-
-////////////////////////////////////////////////////
-// axioms relating Between and BetweenSet
-////////////////////////////////////////////////////
-axiom(forall f: [Loc]Loc, x: Loc, y: Loc, z: Loc :: {knownF(f), known(x), known(y), known(z)} BetweenSet(f, x, z)[y] <==> Between(f, x, y, z));
-axiom(forall f: [Loc]Loc, x: Loc, y: Loc, z: Loc :: {knownF(f), known(x), known(y), known(z)} Between(f, x, y, z) ==> BetweenSet(f, x, z)[y]);
-axiom(forall f: [Loc]Loc, x: Loc :: {knownF(f), known(x)} Between(f, x, x, x));
-axiom(forall f: [Loc]Loc, x: Loc, z: Loc :: {BetweenSet(f, x, z)} Between(f, z, z, z));
-
-
-//////////////////////////
-// Axioms for Between
-//////////////////////////
-
-// reflexive
-axiom(forall f: [Loc]Loc, x: Loc :: Between(f, x, x, x));
-
-// step
-axiom(forall f: [Loc]Loc, x: Loc :: {f[x]} Between(f, x, f[x], f[x]));
-
-// reach
-axiom(forall f: [Loc]Loc, x: Loc, y: Loc :: {f[x], known(y)} Between(f, x, y, y) ==> x == y || Between(f, x, f[x], y));
-
-// cycle
-axiom(forall f: [Loc]Loc, x: Loc, y:Loc :: {f[x], known(y)} f[x] == x && Between(f, x, y, y) ==> x == y);
-
-// sandwich
-axiom(forall f: [Loc]Loc, x: Loc, y: Loc :: {knownF(f), known(x), known(y)} Between(f, x, y, x) ==> x == y);
-
-// order1
-axiom(forall f: [Loc]Loc, x: Loc, y: Loc, z: Loc :: {knownF(f), known(x), known(y), known(z)} Between(f, x, y, y) && Between(f, x, z, z) ==> Between(f, x, y, z) || Between(f, x, z, y));
-
-// order2
-axiom(forall f: [Loc]Loc, x: Loc, y: Loc, z: Loc :: {knownF(f), known(x), known(y), known(z)} Between(f, x, y, z) ==> Between(f, x, y, y) && Between(f, y, z, z));
-
-// transitive1
-axiom(forall f: [Loc]Loc, x: Loc, y: Loc, z: Loc :: {knownF(f), known(x), known(y), known(z)} Between(f, x, y, y) && Between(f, y, z, z) ==> Between(f, x, z, z));
-
-// transitive2
-axiom(forall f: [Loc]Loc, x: Loc, y: Loc, z: Loc, w: Loc :: {knownF(f), known(x), known(y), known(z), known(w)} Between(f, x, y, z) && Between(f, y, w, z) ==> Between(f, x, y, w) && Between(f, x, w, z));
-
-// transitive3
-axiom(forall f: [Loc]Loc, x: Loc, y: Loc, z: Loc, w: Loc :: {knownF(f), known(x), known(y), known(z), known(w)} Between(f, x, y, z) && Between(f, x, w, y) ==> Between(f, x, w, z) && Between(f, w, y, z));
-
-// This axiom is required to deal with the incompleteness of the trigger for the reflexive axiom.
-// It cannot be proved using the rest of the axioms.
-axiom(forall f: [Loc]Loc, u:Loc, x: Loc :: {knownF(f), known(x), known(u)} Between(f, u, x, x) ==> Between(f, u, u, x));
-
-// relation between Avoiding and Between
-axiom(forall f: [Loc]Loc, x: Loc, y: Loc, z: Loc :: {knownF(f), known(x), known(y), known(z)} Avoiding(f, x, y, z) <==> (Between(f, x, y, z) || (Between(f, x, y, y) && !Between(f, x, z, z))));
-axiom(forall f: [Loc]Loc, x: Loc, y: Loc, z: Loc :: {knownF(f), known(x), known(y), known(z)} Between(f, x, y, z) <==> (Avoiding(f, x, y, z) && Avoiding(f, x, z, z)));
-
-// update
-axiom(forall f: [Loc]Loc, u: Loc, v: Loc, x: Loc, p: Loc, q: Loc :: {knownF(f), known(x), known(u), known(v), known(p), known(q)} Avoiding(f[p := q], u, v, x) <==> ((Avoiding(f, u, v, p) && Avoiding(f, u, v, x)) || (Avoiding(f, u, p, x) && p != x && Avoiding(f, q, v, p) && Avoiding(f, q, v, x))));
-
-axiom (forall f: [Loc]Loc, p: Loc, q: Loc, u: Loc, w: Loc :: {knownF(f), known(p), known(q), known(u), known(w)} Avoiding(f, u, w, p) ==> Equal(BetweenSet(f[p := q], u, w), BetweenSet(f, u, w)));
-axiom (forall f: [Loc]Loc, p: Loc, q: Loc, u: Loc, w: Loc :: {knownF(f), known(p), known(q), known(u), known(w)} p != w && Avoiding(f, u, p, w) && Avoiding(f, q, w, p) ==> Equal(BetweenSet(f[p := q], u, w), Union(BetweenSet(f, u, p), BetweenSet(f, q, w))));
-axiom (forall f: [Loc]Loc, p: Loc, q: Loc, u: Loc, w: Loc :: {knownF(f), known(p), known(q), known(u), known(w)} Avoiding(f, u, w, p) || (p != w && Avoiding(f, u, p, w) && Avoiding(f, q, w, p)) || Equal(BetweenSet(f[p := q], u, w), Empty()));
